progs/verif_dotprod.v
@@ -5,22 +5,21 @@ Local Open Scope logic.
 
 Definition add_spec :=
  DECLARE _add
-  WITH n: Z, x: val, y : val, z: val, fy : Z -> float, fz: Z -> float
-  PRE  [_n OF tint, _x OF tptr tdouble, _y OF tptr tdouble, _z OF tptr tdouble] 
-      PROP (0 <= n <= Int.max_signed)
-      LOCAL (`(eq (Vint (Int.repr n))) (eval_id _n);
-                  `(eq x) (eval_id _x);
+  WITH x: val, y : val, z: val, fy : Z -> float, fz: Z -> float
+  PRE  [_x OF tptr tdouble, _y OF tptr tdouble, _z OF tptr tdouble] 
+      PROP ()
+      LOCAL (`(eq x) (eval_id _x);
                   `(eq y) (eval_id _y);
                   `(eq z) (eval_id _z))
-      SEP (`(array_at_ tdouble Tsh 0 n x) ;
-             `(array_at tdouble Tsh (Vfloat oo fy) 0 n y);
-             `(array_at tdouble Tsh (Vfloat oo fz) 0 n z))
+      SEP (`(array_at_ tdouble Tsh 0 3 x) ;
+             `(array_at tdouble Tsh (Vfloat oo fy) 0 3 y);
+             `(array_at tdouble Tsh (Vfloat oo fz) 0 3 z))
   POST [ tvoid ] 
       PROP ()
       LOCAL ()
-      SEP (`(array_at tdouble Tsh (Vfloat oo (fun i => Float.add (fy i) (fz i))) 0 n x);
-             `(array_at tdouble Tsh (Vfloat oo fy) 0 n y);
-             `(array_at tdouble Tsh (Vfloat oo fz) 0 n z) ).
+      SEP (`(array_at tdouble Tsh (Vfloat oo (fun i => Float.add (fy i) (fz i))) 0 3 x);
+             `(array_at tdouble Tsh (Vfloat oo fy) 0 3 y);
+             `(array_at tdouble Tsh (Vfloat oo fz) 0 3 z) ).
 
 Definition dotprod (n: Z) (fx fy : Z -> float) : float :=
   fold_range (fun i sum => Float.add sum (Float.mul (fx i) (fy i)))
@@ -87,7 +86,7 @@ name x_ _x.
 name y_ _y.
 name z_ _z.
 
-forward_for_simple_bound n
+forward_for_simple_bound 3
    (EX i:Z,
       PROP ()
       LOCAL (`(eq x) (eval_id _x);
@@ -95,13 +94,11 @@ forward_for_simple_bound n
                   `(eq z) (eval_id _z))
       SEP (`(array_at tdouble Tsh
                    (fun j => if zlt j i then Vfloat (Float.add (fy j) (fz j)) else Vundef)
-                  0 n x) ;
-             `(array_at tdouble Tsh (Vfloat oo fy) 0 n y);
-             `(array_at tdouble Tsh (Vfloat oo fz) 0 n z))).
+                  0 3 x) ;
+             `(array_at tdouble Tsh (Vfloat oo fy) 0 3 y);
+             `(array_at tdouble Tsh (Vfloat oo fz) 0 3 z))).
 * (* initializer *)
 entailer!.
-unfold array_at_.
-apply array_at_ext'; intros. if_tac; auto. omega.
 * (* body *)
 forward_nl. (* x[i] = y[i] + z[i]; *)
 entailer!.
@@ -110,7 +107,358 @@ unfold upd. if_tac. subst i0. rewrite if_true by omega. auto.
 if_tac. rewrite if_true by omega; auto. rewrite if_false by omega; auto.
 * (*after the for-loop *)
  forward. (*   return; *)
- cancel.
- apply array_at_ext'; intros. rewrite if_true by omega. reflexivity.
 Qed.
+
+Definition Svector_add (n: Z) (_i _x _y _z : ident) :=
+   Ssequence (Sset _i (Econst_int (Int.repr 0) tint))
+     (Sloop
+        (Ssequence
+           (Sifthenelse
+              (Ebinop Olt (Etempvar _i tint) (Econst_int (Int.repr n) tint) tint)
+              Sskip
+              Sbreak)
+           (Sassign
+              (Ederef
+                 (Ebinop Oadd (Etempvar _x (tptr tdouble)) (Etempvar _i tint)
+                    (tptr tdouble)) tdouble)
+              (Ebinop Oadd
+                 (Ederef
+                    (Ebinop Oadd (Etempvar _y (tptr tdouble))
+                       (Etempvar _i tint) (tptr tdouble)) tdouble)
+                 (Ederef
+                    (Ebinop Oadd (Etempvar _z (tptr tdouble))
+                       (Etempvar _i tint) (tptr tdouble)) tdouble) tdouble)))
+        (Sset _i
+           (Ebinop Oadd (Etempvar _i tint) (Econst_int (Int.repr 1) tint)
+              tint))).
+
+Definition vector_add (fx fy: Z -> float) i := 
+    Float.add (fx i) (fy i).
+
+Lemma SEPx_split_rest:
+  forall P Q R1 R,
+   PROPx P (LOCALx Q (SEPx (R1::R))) =
+   PROPx P (LOCALx Q (SEPx (R1::nil))) *PROPx P (LOCALx Q (SEPx R)).
+Proof.
+Admitted.
+
+Lemma replace_nth_commute:
+  forall {A} i j R (a b: A),
+   i <> j ->
+   replace_nth i (replace_nth j R b) a =
+   replace_nth j (replace_nth i R a) b.
+Proof.
+intros.
+rename i into i'. rename j into j'. rename R into R'.
+assert (forall i j R (a b: A),
+             (i<j)%nat -> 
+              replace_nth i (replace_nth j R b) a = replace_nth j (replace_nth i R a) b). {
+induction i; destruct j, R; simpl; intros; auto; try omega.
+f_equal. apply IHi. omega.
+}
+assert (i'<j' \/ i'>j')%nat by omega.
+clear H.
+destruct H1.
+apply H0; auto.
+symmetry; apply H0; auto.
+Qed.
+
+Lemma nth_error_replace_nth':
+  forall {A} i j R (a:A),
+  (i <> j)%nat -> nth_error (replace_nth i R a) j = nth_error R j.
+Proof.
+Admitted.
+Lemma SEPx_drop_rest:
+  forall P Q R1 R,
+   PROPx P (LOCALx Q (SEPx (R1::R))) |--
+   PROPx P (LOCALx Q (SEPx (R1::nil))) * TT.
+Proof.
+Admitted.
+Ltac instantiate_Vptr :=
+  match goal with
+  | H:isptr (eval_id ?i ?rho), A:name ?i
+    |- _ =>
+        let b := fresh "b_" A in
+        let z := fresh "z_" A in
+        let J := fresh "H_" A in
+        destruct (eval_id i rho) as [| | | | b z] eqn:J; try contradiction H;
+         clear H; symmetry in J; rename J into H
+  | H:isptr (eval_id ?i ?rho)
+    |- _ =>
+        let b := fresh "b_"  in
+        let z := fresh "z_"  in
+        let J := fresh "H_"  in
+        destruct (eval_id i rho) as [| | | | b z] eqn:J; try contradiction H;
+         clear H; symmetry in J; rename J into H
+  end.
+
+Lemma semax_vector_add:
+    forall (sx sy sz : nat)
+              (n: Z) Espec Delta P Q R Rx Ry Rz (_i _x _y _z : ident) (x y z: val) (fy fz : Z -> float),
+    typeof_temp Delta _i = Some tint ->
+    Forall (closed_wrt_vars (eq _i)) Q ->
+    Forall (closed_wrt_vars (eq _i)) R ->
+    (0 <= n <= Int.max_signed) ->
+    PROPx P (LOCALx Q (SEPx (TT::nil))) |-- 
+           local (`(eq x) (eval_id _x)) 
+      && local (`(eq y) (eval_id _y)) 
+      && local (`(eq z) (eval_id _z))  ->
+   PROPx P (LOCALx Q (SEPx (Rx::nil))) |-- `(array_at_ tdouble Tsh 0 n x) ->
+   PROPx P (LOCALx Q (SEPx (Ry::nil))) |-- `(array_at tdouble Tsh (Vfloat oo fy) 0 n y) ->
+   PROPx P (LOCALx Q (SEPx (Rz::nil))) |-- `(array_at tdouble Tsh (Vfloat oo fz) 0 n z) ->
+     nth_error R sx = Some Rx ->
+    nth_error R sy = Some Ry ->
+    nth_error R sz = Some Rz ->
+    sx <> sy ->
+    sx <> sz ->  @semax Espec Delta 
+        (PROPx P (LOCALx Q (SEPx R)))
+        (Svector_add n _i _x _y _z)
+        (normal_ret_assert 
+         (PROPx P (LOCALx Q
+          (SEPx  (replace_nth sx R
+             (`(array_at tdouble Tsh (Vfloat oo (vector_add fy fz)) 0 n x))))))).
+Proof.
+intros until 4. intros H6 H7 H8 H9 ? ? ? Nx Ny.
+assert (Ti: (temp_types (initialized _i Delta)) ! _i = Some (tint, true)). {
+clear - H. unfold typeof_temp in H.
+destruct ((temp_types Delta) ! _i) eqn:?; inv H. destruct p.
+inv H1. eapply temp_types_init_same; eauto.
+}
+apply semax_pre0 with
+ (PROPx (isptr x :: isptr y :: isptr z :: P) (LOCALx Q (SEPx R))). {
+repeat rewrite <- canonicalize.canon17.
+repeat rewrite <- andp_assoc. apply andp_right; auto.
+repeat apply andp_right.
+rewrite (replace_nth_nth_error _ _ _ H3).
+erewrite SEP_replace_nth_isolate by (eapply H3).
+apply derives_trans
+  with (PROPx P (LOCALx Q (SEP (Rx))) * SEPx (replace_nth sx R emp));
+ [go_lower; normalize | ].
+eapply derives_trans; 
+  [apply sepcon_derives ; [apply H7 | apply TT_right] | ].
+ unfold array_at_.
+    rewrite array_at_isptr; normalize.
+rewrite (replace_nth_nth_error _ _ _ H4).
+erewrite SEP_replace_nth_isolate by (eapply H4).
+apply derives_trans
+  with (PROPx P (LOCALx Q (SEP (Ry))) * SEPx (replace_nth sy R emp));
+ [go_lower; normalize | ].
+eapply derives_trans; 
+  [apply sepcon_derives ; [apply H8 | apply TT_right] | ].
+    rewrite array_at_isptr; normalize.
+rewrite (replace_nth_nth_error _ _ _ H5).
+erewrite SEP_replace_nth_isolate by (eapply H5).
+apply derives_trans
+  with (PROPx P (LOCALx Q (SEP (Rz))) * SEPx (replace_nth sz R emp));
+ [go_lower; normalize | ].
+eapply derives_trans; 
+  [apply sepcon_derives ; [apply H9 | apply TT_right] | ].
+    rewrite array_at_isptr; normalize.
+}
+repeat rewrite <- canonicalize.canon17.
+apply semax_extract_prop; intro Px.
+apply semax_extract_prop; intro Py.
+apply semax_extract_prop; intro Pz.
+apply (semax_for_simple_bound_const_init n
+   (EX  i : Z, PROPx ((fun _ => P) i)
+                  (LOCALx ((fun _ => Q) i)
+                  (SEPx ((fun i => 
+                 replace_nth sx R
+                   (`(array_at tdouble Tsh (fun j => if zlt j i then Vfloat (Float.add (fy j) (fz j)) else Vundef) 0 n x))
+               ) i))))
+     Espec Delta _ (fun _ => P) (fun _ => Q) (fun i =>  
+                 replace_nth sx R
+                   (`(array_at tdouble Tsh (fun j => if zlt j i then Vfloat (Float.add (fy j) (fz j)) else Vundef) 0 n x))
+               ));
+  try reflexivity; try auto with closed; try repable_signed.
+* 
+intro.
+clear - H1.
+revert R H1.
+induction sx; destruct R; simpl; intros; auto with closed.
+inv H1. auto with closed. inv H1;  constructor; auto with closed.
+*
+apply andp_left2.
+replace (array_at tdouble Tsh
+                 (fun j : Z =>
+                  if zlt j 0
+                  then Vfloat (Float.add (fy j) (fz j))
+                  else Vundef) 0 n)
+ with (array_at_ tdouble Tsh 0 n).
+Focus 2.
+unfold array_at_.
+simple apply array_at_ext; intros.
+rewrite if_false by omega. reflexivity.
+apply derives_trans with 
+  (PROPx P (LOCALx Q (SEPx (replace_nth sx R Rx)))).
+rewrite <- (replace_nth_nth_error _ _ _ H3). auto.
+rewrite <- insert_local.
+apply andp_right.
+go_lowerx; simpl. normalize.
+erewrite SEP_replace_nth_isolate by eassumption.
+erewrite SEP_replace_nth_isolate by eassumption.
+rewrite SEPx_split_rest.
+rewrite (SEPx_split_rest _ _ _ (replace_nth _ _ _)).
+apply sepcon_derives; auto.
+apply andp_right; [apply andp_left1; auto | ].
+apply andp_right; [apply andp_left2; apply andp_left1; auto | ].
+unfold SEPx at 2. unfold fold_right. rewrite sepcon_emp. auto.
+*
+intro i.
+simpl tc_expr.
+go_lowerx; normalize.
+apply prop_right.
+hnf. simpl. 
+rewrite Ti. simpl. apply I.
+*
+rewrite normal_ret_assert_elim.
+simpl update_tycon.
+go_lowerx.
+normalize.
+apply derives_refl'.
+f_equal. f_equal. f_equal. apply equal_f.
+apply array_at_ext; intros.
+rewrite if_true by omega.
+reflexivity.
+*
+intro i.
+match goal with |- semax _ (PROPx ?P (LOCALx ?Q (SEPx ?R))) _ _ =>
+   apply semax_pre0 
+   with (PROPx P (LOCALx (`(eq x) (eval_id _x) :: `(eq y) (eval_id _y) ::
+                           `(eq z) (eval_id _z) :: Q) (SEPx R)))
+ end.
+rewrite <- (insert_local (`(eq _) (eval_id _x))).
+rewrite <- (insert_local (`(eq _) (eval_id _y))).
+rewrite <- (insert_local (`(eq _) (eval_id _z))).
+repeat rewrite <- andp_assoc. apply andp_right; auto.
+rewrite <- insert_local; apply andp_left2.
+rewrite <- insert_local; apply andp_left2.
+repeat rewrite <- canonicalize.canon17; apply andp_left2.
+eapply derives_trans; [ | apply H6].
+apply andp_derives; auto.
+apply andp_derives; auto.
+go_lowerx. rewrite sepcon_emp. apply TT_right.
+apply semax_extract_PROP; intro.
+eapply semax_pre0; [ apply now_later | ].
+eapply semax_post_flipped';
+   [simple eapply (semax_loadstore_array sx);
+       [ reflexivity | apply I | reflexivity | reflexivity| reflexivity 
+       | 
+       | erewrite nth_error_replace_nth; eauto
+       |  |  |  ]
+    |  ].
+match goal with |- (PROPx ?P (LOCALx ?Q (SEPx ?R)))  |-- _ =>
+   set (R' := R)
+end.
+apply derives_trans with
+(PROPx P
+  (LOCALx
+     (`(eq x) (eval_id _x)
+      :: `(eq y) (eval_id _y)
+         :: `(eq z) (eval_id _z)
+            :: `(eq (Vint (Int.repr i))) (eval_id _i)
+               :: `(eq (Vint (Int.repr n)))
+                    (eval_expr (Econst_int (Int.repr n) tint)) :: Q)
+     (SEPx R'))
+   && ((TT * `(array_at tdouble Tsh (Vfloat oo fy) 0 n y))
+     && (TT * `(array_at tdouble Tsh (Vfloat oo fz) 0 n z)))).
+apply andp_right; auto.
+apply andp_right.
+
+repeat (rewrite <- insert_local;  apply andp_left2).
+unfold R'.
+rewrite (replace_nth_nth_error _ _ _ H4).
+rewrite replace_nth_commute by auto.
+
+erewrite SEP_replace_nth_isolate
+ by (rewrite nth_error_replace_nth' by auto; eassumption).
+
+ rewrite sepcon_comm.
+ eapply derives_trans; [apply SEPx_drop_rest | ].
+ apply sepcon_derives; auto.
+
+repeat (rewrite <- insert_local;  apply andp_left2).
+unfold R'.
+rewrite (replace_nth_nth_error _ _ _ H5).
+rewrite replace_nth_commute by auto.
+erewrite SEP_replace_nth_isolate
+ by (rewrite nth_error_replace_nth' by auto; eassumption).
+ rewrite sepcon_comm.
+ eapply derives_trans; [apply SEPx_drop_rest | ].
+ apply sepcon_derives; auto.
+
+go_lowerx.
+unfold R'; clear R'.
+normalize.
+apply andp_left2.
+ subst. repeat instantiate_Vptr; repeat apply andp_right.
+rel_expr.
+rel_expr.
+simple eapply rel_expr_cast; [ | try (simpl; rewrite_eval_id; reflexivity) ].
+simple eapply rel_expr_binop; [ |  | ].
+apply andp_left1. rel_expr.
+apply andp_left2. rel_expr.
+reflexivity.
+reflexivity.
+auto.
+apply I.
+auto.
+
+rewrite replace_nth_replace_nth.
+go_lowerx; normalize.
+apply andp_right.
+ apply prop_right; repeat split; auto; omega.
+apply derives_refl'.
+f_equal. f_equal.
+f_equal.
+apply equal_f.
+apply array_at_ext; intros.
+unfold upd.
+if_tac. subst. rewrite if_true by omega; try reflexivity.
+if_tac.
+rewrite if_true by omega; reflexivity.
+rewrite if_false by omega; reflexivity.
+Qed.
+
+Lemma SEP1_entail:
+  forall P Q R, PROPx P (LOCALx Q (SEP (R))) |-- R.
+Proof.
+intros. apply andp_left2. apply andp_left2.
+go_lowerx. rewrite sepcon_emp; auto.
+Qed.
+
+Ltac forward_seq := 
+  first [eapply semax_seq'; [  | abbreviate_semax ]
+         | eapply semax_post_flipped' ].
+
+Ltac forward_vector_add :=
+ forward_seq;
+ [eapply semax_vector_add;
+   [reflexivity | auto 50 with closed | auto 50 with closed
+   | repable_signed
+   | repeat apply andp_right; go_lowerx; apply prop_right; eauto
+   | try simple apply SEP1_entail
+   | try simple apply SEP1_entail
+   | try simple apply SEP1_entail
+   | try solve_nth_error
+   | try solve_nth_error
+   | try solve_nth_error
+   | computable | computable ]
+ | unfold replace_nth
+ ].
+
+Lemma body_add':  semax_body Vprog Gprog f_add add_spec.
+Proof.
+start_function.
+name i_ _i.
+name x_ _x.
+name y_ _y.
+name z_ _z.
+
+forward_vector_add.
+forward.
+Qed.
+
+
+
 
